Fix various issues

F22.v
@@ -1,3 +1,4 @@
+From Coq Require Import Lia.
 From Coq Require Import Arith.Arith.
 From Coq Require Import Bool.Bool.
 Require Export Coq.Strings.String.
@@ -27,8 +28,8 @@ d. fun (X Y : Type) (x : X) => x
 e. (True, 1)
 f. Some (fun (p : nat * bool) => snd p)
 g. fun (X:Prop) => []
-h. fun (P Q : Prop) => or P Q
-i. something using intro_l and intro r. (*todo proof object*)
+h. empty
+i. fun (P Q : Prop) (p : P) (q : Q) => or_introl p
 *)
 
 End q2.
@@ -41,29 +42,19 @@ Inductive tree :=
     | Empty : tree 
     | Node : nat -> tree -> tree -> tree.
 
-Definition ex_tree_1 : tree := 
-    Node 1 (Node 5 (Node 17 Empty Empty) 
-                    (Node 10 Empty Empty)) 
-            (Node 42 Empty Empty).
-
-Definition ex_tree_2 : tree := 
-    Node 0 
-    (Node 10 Empty Empty) 
-    (Node 5 
-        (Node 2 Empty Empty) 
-        (Node 7 (Node 42 Empty Empty) 
-            (Node 8 Empty Empty))).
+Definition ex_tree_1 : tree := Node 1 (Node 5 (Node 17 Empty Empty) (Node 10 Empty Empty)) (Node 42 Empty Empty).
+Definition ex_tree_2 : tree := Node 0 (Node 10 Empty Empty) (Node 5 (Node 2 Empty Empty) (Node 7 (Node 42 Empty Empty) (Node 8 Empty Empty))).
 
 (* part a *)
 
-(* the exam PDF is incorrect. It should say:: 
-    , the height of ex_tree_1 is 3, while the height of ex_tree_2 is 4.
+(* the exam PDF is incorrect. It should say:
+    the height of ex_tree_1 is 3, while the height of ex_tree_2 is 4.
 
 the max function is OK to assume since it is trivial to implement *)
 Fixpoint height (t: tree) : nat :=  
     match t with
     | Empty => 0
-    | Node v t1 t2 => 1 + max(height t1) (height t2)
+    | Node v t1 t2 => 1 + max (height t1) (height t2)
     end.
 
 (* Trivial tree: *)
@@ -74,12 +65,11 @@ Example height2 : height ex_tree_2 = 4. Proof. reflexivity. Qed.
 
 (* part b *)
 
-(* Check if the treee t is height h or h-1 *)
+(* Helper: check if the tree t is height h or h-1 in all subtrees *)
 Fixpoint is_height (t:tree) (h:nat) : bool :=
 match t, h with
     | Empty, _ => (h <=? 1)
-    | Node x l r , S h' =>
-        andb (is_height l h') (is_height r h')
+    | Node x l r , S h' => andb (is_height l h') (is_height r h')
     | Node x l r, _ => false
 end.
 
@@ -93,6 +83,7 @@ Example balanced1 : balanced ex_tree_1 = true.  Proof. reflexivity. Qed.
 Example balanced2 : balanced ex_tree_2 = false.  Proof. reflexivity. Qed.
 
 (* part c *)
+
 Inductive bal : nat -> tree-> Prop :=
     | Bal_Empty0 : bal 0 Empty
     | Bal_Empty1 : bal 1 Empty
@@ -107,7 +98,12 @@ Example bal_leaf0 : bal 0 Empty. Proof. constructor. Qed.
 Example bal_leaf1 : bal 1 Empty. Proof. constructor. Qed.
 Example bal1 : bal 3 ex_tree_1. Proof. repeat constructor. Qed.
 Example bal2 : forall n, ~ (bal n ex_tree_2). 
-Proof. Admitted.
+Proof. unfold not. intros. inversion H; subst. 
+    inversion H3; subst.
+    inversion H4; subst; inversion H5; subst.
+    - inversion H6.
+    - inversion H9; subst. inversion H8.
+    Qed.
 
 End q3.
 
@@ -116,30 +112,24 @@ End q3.
 Module q4.
 
 (*
-Loop invariant: Y = m * (m - Z) /\ X=m (* TODO: add in the last thing and propogate it thru. it is OK to add more things to the loop invariant like this *)
+Loop invariant: Y = m * (m - Z) /\ X=m 
 
 {{ X = m }} ->> 
-{{ 0 = m * (m - X) }}
+{{ 0 = m * (m - X) /\ X=m }}
     Y := 0; 
-{{ Y = m * (m - X) }}
+{{ Y = m * (m - X) /\ X=m }}
     Z := X;
-{{ Y = m * (m - Z) }}
+{{ Y = m * (m - Z) /\ X=m }}
     WHILE Z > 0 DO 
-{{  Y = m * (m - Z) /\ Z > 0}} ->>
-{{ Y+X = m * (m - (Z-1)) }}
+{{ Y = m * (m - Z) /\ X=m /\ Z > 0 }} ->>
+{{ Y+X = m * (m - (Z-1)) /\ X=m }}
         Z := Z- 1;
-{{ Y+X = m * (m - Z)}}
+{{ Y+X = m * (m - Z) /\ X=m }}
         Y := Y + X
-{{  Y = m * (m - Z) }}
+{{  Y = m * (m - Z) /\ X=m }}
     DONE 
-{{ Y = m * (m - Z) /\ Z <= 0 }} ->>
+{{ Y = m * (m - Z) /\ X=m /\ Z <= 0 }} ->>
 {{ Y = m * m }}
-
-(* this would make sense if we have X=m in the premise, because then we could get
-rid of the +1 and -X from the conclusion *)
-{{  Y = m * (m - Z) /\ Z > 0}} ->>
-{{ Y= m * (m - Z + 1) - X }}
-
 *)
 
 End q4.
@@ -148,15 +138,23 @@ End q4.
 
 Module q5.
 
-(*
-a. 
+(* part a *)
 
+(* Multiple acceptable options:
           
------------------------------- (hoare_assert)
+------------------------------ (hoare_assert_1)
 {{ P }} assert e {{ e /\ P }}
 
-b. 
 
+       P -> b
+-------------------- (hoare_assert_2)
+{{P}} assert b {{P}}
+
+*)
+
+(* part b *)
+
+(*
 | E_AssertTrue
     beval st b = true ->
     st =[ assert e ]=> st
